
\begin{theorem}[Euler's Formula]
\[ e^{i\theta} = \cos(\theta) + i\sin(\theta) \]
\end{theorem}

\begin{proof}
Consider the power series representation of $e^x$:
\[ e^x = \sum_{j=0}^{\infty} \frac{x^j}{j!} \]

Substituting $x = i\theta$, we have
\begin{align*}
e^{i\theta} &= \sum_{j=0}^{\infty} \frac{(i\theta)^j}{j!} \\
&= \sum_{j=0}^{\infty} \frac{(i\theta)^{2j}}{(2j)!} + \sum_{j=0}^{\infty} \frac{(i\theta)^{2j+1}}{(2j+1)!} \tag{separating even and odd terms} \\
&= \sum_{j=0}^{\infty} \frac{i^{2j}\theta^{2j}}{(2j)!} + \sum_{j=0}^{\infty} \frac{i^{2j+1}\theta^{2j+1}}{(2j+1)!} \\
&= \sum_{j=0}^{\infty} \frac{(-1)^j\theta^{2j}}{(2j)!} + i\sum_{j=0}^{\infty} \frac{(-1)^j\theta^{2j+1}}{(2j+1)!} \tag{since $i^{2j} = (-1)^j$ and $i^{2j+1} = i(-1)^j$} \\
&= \cos(\theta) + i\sin(\theta)
\end{align*}

The last equality follows from the Taylor series expansions:
\[ \cos(\theta) = \sum_{j=0}^{\infty} \frac{(-1)^j\theta^{2j}}{(2j)!} \quad \text{and} \quad \sin(\theta) = \sum_{j=0}^{\infty} \frac{(-1)^j\theta^{2j+1}}{(2j+1)!} \]

Note that this manipulation is justified by the absolute convergence of the exponential series for all complex numbers.
\end{proof}








